experiments/meta/Criteria2.fst
@@ -1,0 +1,91 @@
+module Criteria2
+
+(** *** Intrinsic criteria, static quoting/unquoting  **)
+
+type set_prop = int -> Type0
+let (⊆) (s0 s1:set_prop) : Type0 = forall res. s0 res ==> s1 res
+let (≡) (s0 s1:set_prop) : Type0 = forall res. s0 res <==> s1 res
+
+noeq type intS = { ct : Type u#a; p_post : set_prop }
+
+type progS (i:intS) = i.ct -> Pure int True i.p_post
+type ctxS (i:intS) = i.ct
+type wholeS = post:set_prop & (unit -> Pure int True post)
+
+let linkS (#i:intS) (ps:progS i) (cs:ctxS i) : wholeS =
+  (| i.p_post, (fun () -> ps cs) |)
+
+assume type pure_repr
+assume val reify' : (unit -> Pure int True (fun _ -> True)) -> pure_repr
+assume val behS0 : pure_repr -> set_prop
+
+val behS : wholeS -> set_prop 
+let behS (| _, ws |) = behS0 (reify' ws)
+
+(** Target **)
+assume type ast
+assume type ast_typ
+assume type ast_env
+assume type ast_typing (g:ast_env) (a:ast) (t:ast_typ)
+
+noeq type intT = { ct : ast_typ; g : ast_env; }
+
+assume val comp_int : intS u#a -> ast_env -> intT
+
+// TODO: g does not appear hear
+type progT (i:intT) = pt:ast//{ast_typing i.g pt ...}
+type ctxT (i:intT) = ct:ast//{ast_typing i.g ct ...}
+type wholeT = wt:ast_typ//{ast_typing i.g wt ...}
+
+assume val linkT (#i:intT) (pt:progT i) (ct:ctxT i) : wholeT
+
+assume val behT : wt:wholeT -> set_prop 
+
+open FStar.Tactics.V2
+open FStar.Reflection.V2
+open FStar.Reflection.Typing
+let mk_squash (phi:term) : Tot term = pack_ln (Tv_App (`squash) (phi, Q_Explicit))
+
+let t_unit = `()
+
+let valid (g:env) (phi:term) : prop =
+  squash (tot_typing g t_unit (mk_squash phi))
+
+// TODO: (`wholeS) elaborates to FVar, so we need to unfold that to get the type
+val compile_whole_stat : 
+  (g:env) ->
+  (ws:term{tot_typing g ws (`wholeS)}) ->
+  (g_ast : term{tot_typing g g_ast (`ast_env)}) ->
+  Tac (wt:term{
+    tot_typing g wt (`wholeT) /\
+    (** compiler correctness **)
+    valid g (`(behS (`#ws) ≡ behT (`#wt)))
+
+    (** soundness **)
+    // in this PoC, we cannot type this because whole programs do not have an interface
+    // valid g (`(behT (`#wt) ⊆ i.p_post))
+  })
+
+let soundness (#i:intS) (#g_ast:ast_env) (pt:progT (comp_int i g_ast)) =
+  forall (ct:ctxT (comp_int i g_ast)). behT (linkT pt ct) ⊆ i.p_post
+
+(** The order of the quantifiers makes this RHC (Robust Hyperproperty Preservation) **)
+(** TODO: why cannot we change the order of the quantifiers to have RrHC **)
+let rhc (#i:intS) (#g_ast:ast_env) (ps:progS i) (pt:progT (comp_int i g_ast)) =
+  forall (ct:ctxT (comp_int i g_ast)).
+    exists (cs:ctxS i). behS (linkS ps cs) ≡ behT (linkT pt ct)
+
+val compile_prog_soundness :
+  (g:env) ->
+  #i:term{tot_typing g i (`intS)} ->
+  ps:term{tot_typing g ps (`progS (`#i))} ->
+  (g_ast : term{tot_typing g g_ast (`ast_env)}) ->
+  Tac (pt:term{
+    tot_typing g pt (`progT (comp_int (`#i) (`#g_ast))) /\
+
+    (** soundness **)
+    valid g (`(soundness (`#pt))) /\
+
+    (** RHC **)
+    valid g (`(rhc (`#ps) (`#pt)))
+  })
